with all the options

AwsCryptographicMaterialProviders/dafny/AwsCryptographyKeyStore/src/Structure.dfy
@@ -73,10 +73,49 @@ module {:options "/functionSyntax:4" } Structure {
     || s == MUTATION_INDEX_TYPE
   }
 
+  lemma NoRestrictedAttributeNameStartsWithPrefix()
+    ensures (
+              forall
+                reserved <- BRANCH_KEY_RESTRICTED_FIELD_NAMES
+                ::
+                  !( ENCRYPTION_CONTEXT_PREFIX <= reserved) && !(ENCRYPTION_CONTEXT_PREFIX < reserved)
+            )
+  {
+    //HierarchyVersionIsNotPrefixed();
+    assert && ENCRYPTION_CONTEXT_PREFIX[0] as char == 'a' as char
+           && HIERARCHY_VERSION[0] == 'h'
+           && "a" != "h";
+  }
+
+  // lemma RestrictedStringsAreNotPrefixed(s: string)
+  //   ensures s in BRANCH_KEY_RESTRICTED_FIELD_NAMES ==> !(ENCRYPTION_CONTEXT_PREFIX <= s)
+  // {
+  //   assert && ENCRYPTION_CONTEXT_PREFIX[0] == 'a'
+  //          && HIERARCHY_VERSION[0] == 'h'
+  //          && 'a' != 'h';
+  // }
+
+  lemma RestrictedStringsEnsureNotPrefixed(s: string)
+    requires s in BRANCH_KEY_RESTRICTED_FIELD_NAMES
+    ensures !(ENCRYPTION_CONTEXT_PREFIX <= s)
+  {
+    assert && ENCRYPTION_CONTEXT_PREFIX[0] == 'a'
+           && HIERARCHY_VERSION[0] == 'h'
+           && 'a' != 'h';
+  }
+
+  // lemma HierarchyVersionIsNotPrefixed()
+  //   ensures && ENCRYPTION_CONTEXT_PREFIX[0] as char == 'a' as char
+  //           && HIERARCHY_VERSION[0] == 'h'
+  //           && "a" != "h"
+  // {}
+
   type PrefixedEncryptionContext = m: map<string, string> | PrefixedEncryptionContext?(m) witness *
-  predicate PrefixedEncryptionContext?(m: map<string, string>) {
-    && m.Keys !! BRANCH_KEY_RESTRICTED_FIELD_NAMES
-    && forall k :: k in m.Keys ==> ENCRYPTION_CONTEXT_PREFIX <= k
+  predicate PrefixedEncryptionContext?(m: map<string, string>): (output: bool)
+    ensures output ==> m.Keys !! BRANCH_KEY_RESTRICTED_FIELD_NAMES
+  {
+    // && m.Keys !! BRANCH_KEY_RESTRICTED_FIELD_NAMES
+    forall k :: k in m.Keys ==> ENCRYPTION_CONTEXT_PREFIX <= k
   }
 
   predicate StringIsValidHierarchyVersion?(version: string)
@@ -427,7 +466,7 @@ module {:options "/functionSyntax:4" } Structure {
     var prefixKeys := set k <- encryptionContext.Keys | ENCRYPTION_CONTEXT_PREFIX <= k;
 
     // Dafny needs some help.
-    // Adding a fixed string
+    // Removing a fixed string
     // will not make any of the keys collide.
     assert forall k <- prefixKeys ::
         k == ENCRYPTION_CONTEXT_PREFIX + k[|ENCRYPTION_CONTEXT_PREFIX|..];
@@ -444,55 +483,6 @@ module {:options "/functionSyntax:4" } Structure {
             Types.KeyStoreException( message :="Unable to encode string"));
 
     Success(map i <- encodedEncryptionContext :: i.0.value := i.1.value)
-  }
-
-  /** Selects the key-value pairs prefixed with ENCRYPTION_CONTEXT_PREFIX **/
-  function SelectCustomEncryptionContextAsString(
-    encryptionContext: Types.EncryptionContextString
-  ): (output: Types.EncryptionContextString)
-    ensures forall k <- output
-              ::
-                (|k| > |ENCRYPTION_CONTEXT_PREFIX|)
-                && k[ .. |ENCRYPTION_CONTEXT_PREFIX|] == ENCRYPTION_CONTEXT_PREFIX
-                && (k in encryptionContext)
-                && encryptionContext[k] == output[k]
-    ensures BRANCH_KEY_RESTRICTED_FIELD_NAMES !! output.Keys
-  {
-    var customKeys
-      :=
-      set k <- encryptionContext
-          | ENCRYPTION_CONTEXT_PREFIX < k && (|k| > |ENCRYPTION_CONTEXT_PREFIX|)
-            && k[0] == ENCRYPTION_CONTEXT_PREFIX[0]
-            // //It really helps Dafny to have a specific check
-        ::
-          // assert HIERARCHY_VERSION != k by {assert k[0] != HIERARCHY_VERSION[0];}
-          k;
-    map i <- customKeys :: i := encryptionContext[i]
-  }
-
-  function ExtractCustomEncryptionContextAs(
-    encryptionContext: BranchKeyContext
-  ): (output: Types.EncryptionContextString)
-    ensures
-      forall k <- output
-        ::
-          && (ENCRYPTION_CONTEXT_PREFIX + k in encryptionContext)
-          && encryptionContext[ENCRYPTION_CONTEXT_PREFIX + k] == output[k]
-  {
-    // Dafny needs some help.
-    // Adding a fixed string
-    // will not make any of the keys collide.
-    assert forall k <- encryptionContext.Keys | ENCRYPTION_CONTEXT_PREFIX < k
-        ::
-          k == ENCRYPTION_CONTEXT_PREFIX + k[|ENCRYPTION_CONTEXT_PREFIX|..];
-
-    var defixedCustomEncryptionContext
-      := set k <- encryptionContext
-             | ENCRYPTION_CONTEXT_PREFIX < k
-           ::
-             (k[|ENCRYPTION_CONTEXT_PREFIX|..], encryptionContext[k]);
-
-    map i <- defixedCustomEncryptionContext :: i.0 := i.1
   }
 
   opaque function DecryptOnlyBranchKeyEncryptionContext(
@@ -512,7 +502,7 @@ module {:options "/functionSyntax:4" } Structure {
     ensures output[KMS_FIELD] == kmsKeyArn
     ensures output[TABLE_FIELD] == logicalKeyStoreName
     ensures output[HIERARCHY_VERSION] == HierarchyVersionToString(hierarchyVersion)
-    ensures forall k <- encryptionContext
+    ensures forall k <- encryptionContext.Keys
               ::
                 && ENCRYPTION_CONTEXT_PREFIX + k in output
                 && output[ENCRYPTION_CONTEXT_PREFIX + k] == encryptionContext[k]
@@ -533,17 +523,40 @@ module {:options "/functionSyntax:4" } Structure {
     // I would like to make some tiny functions that handle just prefixing...
     var prefixedEncryptionContext :=
       map k <- encryptionContext :: ENCRYPTION_CONTEXT_PREFIX + k := encryptionContext[k];
-    assume {:axiom} forall k :: k in prefixedEncryptionContext.Keys ==> ENCRYPTION_CONTEXT_PREFIX < k;
-    assume {:axiom} prefixedEncryptionContext.Keys !! BRANCH_KEY_RESTRICTED_FIELD_NAMES;
-    assert PrefixedEncryptionContext?(prefixedEncryptionContext);
-    prefixedEncryptionContext + map[
-      BRANCH_KEY_IDENTIFIER_FIELD := branchKeyId,
-      TYPE_FIELD := BRANCH_KEY_TYPE_PREFIX + branchKeyVersion,
-      KEY_CREATE_TIME := timestamp,
-      TABLE_FIELD := logicalKeyStoreName,
-      KMS_FIELD := kmsKeyArn,
-      HIERARCHY_VERSION := HierarchyVersionToString(hierarchyVersion)
-    ]
+    // assume {:axiom} forall k :: k in prefixedEncryptionContext.Keys ==> ENCRYPTION_CONTEXT_PREFIX <= k;
+    // assume {:axiom} prefixedEncryptionContext.Keys !! BRANCH_KEY_RESTRICTED_FIELD_NAMES;
+    assert
+      (
+        (forall k :: k in prefixedEncryptionContext.Keys
+                     ==>
+                       ENCRYPTION_CONTEXT_PREFIX <= k)
+        &&
+        (
+          forall
+            reserved <- BRANCH_KEY_RESTRICTED_FIELD_NAMES
+            ::
+              !( ENCRYPTION_CONTEXT_PREFIX <= reserved) && !(ENCRYPTION_CONTEXT_PREFIX < reserved)
+        )
+        ==> PrefixedEncryptionContext?(prefixedEncryptionContext)
+      );
+    assert forall k <- encryptionContext.Keys
+        ::
+          && ENCRYPTION_CONTEXT_PREFIX + k in prefixedEncryptionContext
+          && prefixedEncryptionContext[ENCRYPTION_CONTEXT_PREFIX + k] == encryptionContext[k];
+
+    var output := prefixedEncryptionContext + map[
+                    BRANCH_KEY_IDENTIFIER_FIELD := branchKeyId,
+                    TYPE_FIELD := BRANCH_KEY_TYPE_PREFIX + branchKeyVersion,
+                    KEY_CREATE_TIME := timestamp,
+                    TABLE_FIELD := logicalKeyStoreName,
+                    KMS_FIELD := kmsKeyArn,
+                    HIERARCHY_VERSION := HierarchyVersionToString(hierarchyVersion)
+                  ];
+    assert forall k <- encryptionContext.Keys
+        ::
+          && ENCRYPTION_CONTEXT_PREFIX + k in prefixedEncryptionContext
+          && output[ENCRYPTION_CONTEXT_PREFIX + k] == encryptionContext[k];
+    output
   }
 
   function ActiveBranchKeyEncryptionContext(
